Okay, this is how equality has to look like. Sliightly more complicated.

thy/OpenFlow/FeatherweightOpenFlowComparison.thy
@@ -4,10 +4,10 @@ begin
 
 (* compare to https://github.com/frenetic-lang/featherweight-openflow/blob/master/coq/OpenFlow/OpenFlowSemantics.v#L260 *)
 inductive guha_table_semantics :: "('m, 'p) field_matcher \<Rightarrow> ('m, 'a) flowtable \<Rightarrow> 'p \<Rightarrow> 'a option \<Rightarrow> bool" where
-"\<gamma> (ofe_fields fe) p = True \<Longrightarrow> 
+guha_matched: "\<gamma> (ofe_fields fe) p = True \<Longrightarrow> 
  \<forall>fe' \<in> set (ft1 @ ft2). ofe_prio fe' > ofe_prio fe \<longrightarrow> \<gamma> (ofe_fields fe') p = False \<Longrightarrow> 
  guha_table_semantics \<gamma> (ft1 @ fe # ft2) p (Some (ofe_action fe))" |
-"\<forall>fe \<in> set ft. \<gamma> (ofe_fields fe) p = False \<Longrightarrow>
+guha_unmatched: "\<forall>fe \<in> set ft. \<gamma> (ofe_fields fe) p = False \<Longrightarrow>
  guha_table_semantics \<gamma> ft p None"
 
 (* 
@@ -47,6 +47,20 @@ proof -
 	done
 qed
 
+lemma guha_matched_rule_inversion:
+	assumes "guha_table_semantics \<gamma> ft p (Some a)"
+	shows "\<exists>fe \<in> set ft. a = ofe_action fe \<and> \<gamma> (ofe_fields fe) p \<and> (\<forall>fe' \<in> set ft. ofe_prio fe' > ofe_prio fe \<longrightarrow> \<not>\<gamma> (ofe_fields fe') p)"
+proof - 
+	{
+		fix d
+		assume "guha_table_semantics \<gamma> ft p d"
+		hence "Some a = d \<Longrightarrow> (\<exists>fe \<in> set ft. a = ofe_action fe \<and> \<gamma> (ofe_fields fe) p \<and> (\<forall>fe' \<in> set ft. ofe_prio fe' > ofe_prio fe \<longrightarrow> \<not>\<gamma> (ofe_fields fe') p))"
+			by(induction rule: guha_table_semantics.induct) simp_all (* strange to show this by induction, but I don't see an exhaust or cases I could use. *)
+	}
+	from this[OF assms refl]
+	show ?thesis .
+qed
+
 lemma guha_equal_Action:
 	assumes no: "no_overlaps \<gamma> ft"
 	assumes spm: "OF_same_priority_match3 \<gamma> ft p = Action a"
@@ -69,14 +83,44 @@ lemma guha_equal_NoAction:
 using spm unfolding OF_same_priority_match3_def
 by(auto simp add: filter_empty_conv OF_spm3_noa_none[OF no spm] intro: guha_table_semantics.intros(2) split: list.splits)
 
-lemma
+lemma guha_equal:
 	assumes no: "no_overlaps \<gamma> ft"
 	shows "guha_table_semantics \<gamma> ft p (ftb_to_option (OF_same_priority_match3 \<gamma> ft p))"
-unfolding ftb_to_option_def
+	unfolding ftb_to_option_def
 	apply(cases "(OF_same_priority_match3 \<gamma> ft p)")
 	apply(simp add: guha_equal_Action[OF no])
 	apply(simp add: guha_equal_NoAction[OF no])
 	apply(subgoal_tac False, simp)
-	using check_no_overlapI no no_overlap_not_unefined no_overlaps_defeq by fastforce
+	apply(simp add: no no_overlaps_not_unefined)
+done
+
+lemma guha_deterministic1: "guha_table_semantics \<gamma> ft p (Some x1) \<Longrightarrow> \<not> guha_table_semantics \<gamma> ft p None" by (metis Some_helper guha_table_semantics.simps in_set_conv_decomp)
+lemma guha_deterministic2: "\<lbrakk>no_overlaps \<gamma> ft; guha_table_semantics \<gamma> ft p (Some x1); guha_table_semantics \<gamma> ft p (Some a)\<rbrakk> \<Longrightarrow> x1 = a"
+proof(rule ccontr)
+	case goal1
+	note goal1(2-3)[THEN guha_matched_rule_inversion] then obtain fe1 fe2 where fes:
+	"fe1\<in>set ft" "x1 = ofe_action fe1" "\<gamma> (ofe_fields fe1) p" "(\<forall>fe'\<in>set ft. ofe_prio fe1 < ofe_prio fe' \<longrightarrow> \<not> \<gamma> (ofe_fields fe') p)"
+    "fe2\<in>set ft" "a  = ofe_action fe2" "\<gamma> (ofe_fields fe2) p" "(\<forall>fe'\<in>set ft. ofe_prio fe2 < ofe_prio fe' \<longrightarrow> \<not> \<gamma> (ofe_fields fe') p)"
+    	by blast
+    from `x1 \<noteq> a` have fene: "fe1 \<noteq> fe2" using fes(2,6) by blast
+    have pe: "ofe_prio fe1 = ofe_prio fe2" using fes(1,3-4,5,7-8) less_linear by blast
+    note `no_overlaps \<gamma> ft`[THEN check_no_overlapI, unfolded check_no_overlap_def]
+    note this[unfolded Ball_def, THEN spec, THEN mp, OF fes(1), THEN spec, THEN mp, OF fes(5),THEN spec, THEN mp, OF UNIV_I, of p] pe fene fes(3,7)
+    thus False by blast
+qed
+
+lemma guha_equal2:
+	assumes no: "no_overlaps \<gamma> ft"
+	shows "OF_same_priority_match3 \<gamma> ft p = option_to_ftb d \<longleftrightarrow> guha_table_semantics \<gamma> ft p d"
+	unfolding option_to_ftb_def
+	using guha_equal[OF no, of p] unfolding ftb_to_option_def option_to_ftb_def
+	apply(cases "OF_same_priority_match3 \<gamma> ft p"; cases d)
+	apply(simp_all)
+	using guha_deterministic1 apply fast
+	using guha_deterministic2[OF no] apply blast
+	using guha_deterministic1 apply fast
+	using no_overlaps_not_unefined[OF no] apply fastforce
+	using no_overlaps_not_unefined[OF no] apply fastforce 
+done
 
 end
